skip_list/spec/insert.v
@@ -18,119 +18,19 @@ Module AddSpec (Params: SKIP_LIST_PARAMS).
   Section Proofs.
     Context `{!heapGS Σ, !gset_list_unionGS Σ, !lockG Σ} (lvlN : namespace).
 
-    Theorem findLock_spec (head curr: node_rep) (key: Z)
-      (Γ: lazy_gname) (P: node_rep → iProp Σ) :
-      {{{ 
-        inv lvlN (lazy_list_inv head Γ P)
-        ∗
-        (⌜ curr = head ⌝ ∨ own (s_auth Γ) (◯ {[curr]}))
-        ∗
-        ⌜ node_key curr < key < INT_MAX ⌝
-      }}}
-        findLock (rep_to_node curr) #key
-      {{{ pred succ, RET SOMEV ((rep_to_node pred), (rep_to_node succ));
-        ⌜ node_key pred < key ≤ node_key succ ⌝
-        ∗
-        (⌜ pred = head ⌝ ∨ own (s_auth Γ) (◯ {[pred]}))
-        ∗
-        (own (s_auth Γ) (◯ {[succ]}) ∨ ⌜ succ = tail ⌝)
-        ∗
-        ∃ (l: loc) (γ: gname), ⌜ node_next pred = Some l ⌝
-                               ∗
-                               is_lock γ (node_lock pred) (node_inv l)
-                               ∗
-                               l ↦{#1 / 2} (rep_to_node succ)
-                               ∗
-                               locked γ
-      }}}.
-    Proof.
-      iIntros (Φ) "(#Hinv & Hown_curr & Hrange) HΦ".
-      iRevert (curr) "Hown_curr Hrange".
-      iLöb as "IH". 
-      iIntros (curr) "#Hown_curr %Hrange".
-      
-      wp_lam. wp_let.
-      wp_apply (find_frac_spec with "[Hown_curr]").
-      { by iFrame "#". }
-      iIntros (pred succ) "(%Hrange' & #Hown_pred & #Hown_succ & Hlock)".
-      iDestruct "Hlock" as (l γ) "(%Hsome & #Hlock)".
-      wp_pures. wp_lam. wp_pures.
-
-      wp_bind (acquire _).
-      iApply (acquire_spec with "Hlock"); first done.
-      iNext; iIntros (v) "(Hnode & Hlocked)".
-      wp_pures. wp_lam. wp_pures.
-      rewrite Hsome; wp_match.
-      iDestruct "Hnode" as (rep) "Hnode".
-
-      wp_bind (Load _).
-      iInv lvlN as (S L) "(>%Hperm & >%Hsort & Hown_auth & Hown_frac & Hlist)" "Hclose".
-
-      iMod "Hown_auth"; iAssert ⌜ pred = head ∨ In pred L ⌝%I
-        with "[Hown_auth Hown_pred]" as %Hpred_range.
-      {
-        iDestruct "Hown_pred" as "[Heq|Hown]"; first by iLeft.
-        iDestruct (own_valid_2 with "Hown_auth Hown") 
-          as %[Hvalid%gset_included]%auth_both_valid_discrete.
-        iPureIntro; right. 
-        rewrite -elem_of_list_In Hperm elem_of_elements.
-        set_solver.
-      }
-
-      iAssert ⌜ In succ L ∨ succ = tail ⌝%I
-        with "[Hown_auth Hown_succ]" as %Hsucc_range.
-      {
-        iDestruct "Hown_succ" as "[Hown|Heq]"; last by iRight.
-        iDestruct (own_valid_2 with "Hown_auth Hown") 
-          as %[Hvalid%gset_included]%auth_both_valid_discrete.
-        iPureIntro; left. 
-        rewrite -elem_of_list_In Hperm elem_of_elements.
-        set_solver.
-      }
-
-      rewrite (list_equiv_invert L head pred); last done.
-      iDestruct "Hlist" as (succ' ? ? l' γ') "(>%Hsucc'_in_L & _ & >%Hsome' & Hpt & _ & Himp)".
-      assert (l = l') as <- by congruence.
-
-      wp_load.
-      iDestruct (mapsto_agree with "Hnode Hpt") as "%Hsucc".
-      assert (rep = succ') as -> by by apply rep_to_node_inj.
-      iMod ("Hclose" with "[Hpt Himp Hown_auth Hown_frac]").
-      {
-        iNext. iExists S, L.
-        iPoseProof ("Himp" with "Hpt") as "Hlist".
-        by iFrame.
-      }
-
-      iModIntro. wp_let. wp_lam. wp_pures. wp_lam. wp_pures.
-      case_bool_decide as Heq; wp_if.
-      + wp_pures. iApply "HΦ". iModIntro; iFrame "# ∗".
-        iSplit. done. iExists l, γ.
-        assert (succ = succ') as <-; last by iFrame "# ∗".
-        apply (sorted_node_key_unique (L ++ [tail])).
-        - apply node_rep_sorted_app in Hsort; by destruct Hsort.
-        - by rewrite in_inv_rev.
-        - by rewrite in_inv_rev. 
-        - congruence.
-      + wp_lam. wp_pures.
-        wp_apply (release_spec with "[Hnode Hlocked]"); first done.
-        { iFrame "# ∗"; iExists succ'; iFrame. }
-        iIntros. wp_pures.
-        by iApply ("IH" with "HΦ").
-    Qed.
-
     Theorem tryInsert_spec (curr head: node_rep) (key: Z) 
-      (q: frac) (Skeys: gset Z) (Γ: lazy_gname) :
+      (q: frac) (Skeys: gset Z) (bot: lazy_gname) :
+      INT_MIN < key < INT_MAX →
       {{{
-        is_lazy_list lvlN head q Skeys Γ from_bot_list
+        is_lazy_list lvlN head q Skeys bot from_bot_list
         ∗
-        (⌜ curr = head ⌝ ∨ own (s_auth Γ) (◯ {[curr]}))
+        (⌜ curr = head ⌝ ∨ own (s_auth bot) (◯ {[ curr ]}))
         ∗
-        ⌜ node_key curr < key < INT_MAX ⌝
+        ⌜ node_key curr < key ⌝
       }}}
         tryInsert (rep_to_node curr) #key
       {{{ v new, RET v;
-        is_lazy_list lvlN head q (Skeys ∪ {[key]}) Γ from_bot_list
+        is_lazy_list lvlN head q (Skeys ∪ {[ key ]}) bot from_bot_list
         ∗
         ( 
           ⌜ v = NONEV ⌝ ∨ 
@@ -138,41 +38,43 @@ Module AddSpec (Params: SKIP_LIST_PARAMS).
             ⌜ v = SOMEV (rep_to_node new) ⌝ 
             ∗ 
             ⌜ node_key new = key ⌝
+            ∗ 
+            own (s_auth bot) (◯ {[ new ]})
+            ∗ 
+            own (s_toks bot) (GSet {[ node_key new ]})
           )
         )
       }}}.
     Proof.
-      iIntros (Φ) "(Hlazy & #Hown_curr & %Hrange) HΦ".
+      iIntros (Hkey_range Φ) "(Hlazy & #Hown_curr & %Hrange) HΦ".
       iDestruct "Hlazy" as (Sfrag) "(%Hequiv & Hown_frag & #Hinv)".
       wp_lam. wp_let.
 
       wp_apply findLock_spec.
-      { by iFrame "#". }
+      { iFrame "#". iPureIntro; lia. }
       iIntros (pred succ) "(%Hrange' & #Hown_pred & #Hown_succ & Hlock)".
       iDestruct "Hlock" as (l γ) "(%Hsome & #Hlock & Hpt & Hlocked)".
 
       wp_pures. wp_lam. wp_pures.
       case_bool_decide as Hcase; wp_if.
-      + iDestruct "Hown_succ" as "[Hown_succ|%Hsucc]"; last first.
-        { 
-          subst; exfalso. inversion Hcase as [Heq]. 
-          rewrite /node_key/tail//= in Heq; lia. 
-        }
+      + assert (key = node_key succ) as Heq by congruence.
+        iDestruct "Hown_succ" as "[Hown_succ|%Hsucc]"; last first.
+        { subst; exfalso. rewrite /node_key/tail/= in Hkey_range; lia. }
 
         wp_lam. wp_bind (Snd _).
-        iInv lvlN as (S L) "(>%Hperm & >%Hsort & Hown_auth & Hown_frac & Hlist)" "Hclose".
-        iMod "Hown_auth"; iDestruct (own_valid_2 with "Hown_auth Hown_succ") 
+        iInv lvlN as (S Skeys' L) "(>%Hperm & >%Hsort &>%Hequiv' & >Hown_auth & >Hown_frac & >Hown_toks & Hlist)" "Hclose".
+        iDestruct (own_valid_2 with "Hown_auth Hown_succ") 
           as %[Hvalid%gset_included]%auth_both_valid_discrete.
-        iMod "Hown_frac"; iDestruct (own_valid_2 with "Hown_frac Hown_frag") 
+        iDestruct (own_valid_2 with "Hown_frac Hown_frag") 
           as %Hsub%frac_auth_included_total%gset_included.
         iMod (own_update_2 with "Hown_frac Hown_frag") as "[Hown_frac Hown_frag]".
         { apply frac_auth_update, (gset_local_update_union _ _ {[ succ ]}). }
 
-        wp_pures.
-        iMod ("Hclose" with "[Hlist Hown_auth Hown_frac]") as "_".
+        wp_proj.
+        iMod ("Hclose" with "[Hlist Hown_auth Hown_frac Hown_toks]") as "_".
         {
-          iNext. iExists S, L.
-          assert (S ∪ {[ succ ]} ≡ S) as -> by set_solver.
+          iNext; iExists S, Skeys', L.
+          assert (S = S ∪ {[ succ ]}) as <- by set_solver.
           by iFrame.
         }
         iModIntro.
@@ -180,39 +82,32 @@ Module AddSpec (Params: SKIP_LIST_PARAMS).
         wp_apply (release_spec with "[Hlock Hpt Hlocked]"); first done.
         { iFrame "# ∗"; iExists succ; iFrame. }
         iIntros "_". wp_pures.
-        iModIntro. iApply "HΦ".
-        iSplit; last by iLeft.
-        iExists (Sfrag ∪ {[succ]}). 
+        iModIntro. iApply ("HΦ" $! _ succ).
+        iSplitR ""; last by iLeft.
+        iExists (Sfrag ∪ {[ succ ]}). 
         iFrame "# ∗". iPureIntro.
 
-        assert (key = node_key succ) as -> by congruence.
-        assert (key_equiv {[ succ ]} {[ node_key succ ]}) as Hequiv''.
-        { rewrite /key_equiv ?elements_singleton //. }
-
-        assert (Sfrag ∪ {[ succ ]} ⊆ S) as Hsub_union_S.
+        eapply key_equiv_union.
+        { done. }
+        { by do 2 apply node_rep_sorted_app in Hsort as [? Hsort]. }
+        { done. }
+        { rewrite Heq /key_equiv ?elements_singleton //. }
         { by apply union_subseteq. }
-
-        apply node_rep_sorted_app in Hsort as [_ Hsort].
-        apply node_rep_sorted_app in Hsort as [Hsort _].
-
-        by apply (key_equiv_union L S Sfrag {[ succ ]} Skeys {[ node_key succ ]}).
       + wp_lam. wp_pures.
         rewrite Hsome; wp_match.
         wp_load. wp_let. wp_alloc l' as "Hpt'". wp_let.
         iDestruct "Hpt'" as "(Hpt' & Hpt'_dup)".
-
-        assert (key ≠ node_key succ) as Hneq by congruence.
         
         wp_apply (newlock_spec (node_inv l') with "[Hpt'_dup]").
         { iExists succ; iFrame. }
         iIntros (lk) "#Hlock'". iDestruct "Hlock'" as (γ') "Hlock'".
 
-        wp_bind (InjR _).
-        iInv lvlN as (S L) "(>%Hperm & >%Hsort & Hown_auth & Hown_frac & Hlist)" "Hclose".
+        wp_pures.
+        rewrite (fold_rep_to_node (key, Some l', None, lk)).
+        set (new := (key, Some l', None, lk)).
         
-        wp_inj.
-        iDestruct (own_valid_2 with "Hown_frac Hown_frag") 
-          as %HsubS%frac_auth_included_total%gset_included.
+        wp_bind (Store _ _).
+        iInv lvlN as (S Skeys' L) "(>%Hperm & >%Hsort & >%Hequiv' & >Hown_auth & >Hown_frac & >Hown_toks & Hlist)" "Hclose".
 
         iAssert ⌜ pred = head ∨ In pred L ⌝%I
           with "[Hown_auth Hown_pred]" as %Hpred_range.
@@ -225,16 +120,34 @@ Module AddSpec (Params: SKIP_LIST_PARAMS).
           set_solver.
         }
 
-        iAssert ⌜ key ∉ Skeys ⌝%I
-          with "[Hlist Hpt Hown_auth Hown_pred]" as %Hnin.
-        {
-          rewrite (list_equiv_invert L head pred); last done.
-          iDestruct "Hlist" as (succ'' L1 L2 l'' γ'') "(_ & %Hsplit & %Hsome'' & Hpt'' & _)".
-          assert (l = l'') as <- by congruence.
-          iDestruct (mapsto_agree with "Hpt Hpt''") as %Hsucc.
-          iPureIntro.
-          apply rep_to_node_inj in Hsucc. rewrite -Hsucc in Hsplit.
+        assert (key ≠ node_key succ) as Hneq by congruence.
+        rewrite (list_equiv_insert head pred new succ L l l' γ'); first last.
+        { done. }
+        { auto. }
+        { assert (node_key new = key) as -> by auto; lia. }
+        { rewrite /node_key/=; lia. }
 
+        iDestruct ("Hlist" with "[Hpt Hpt' Hlock]") as "Hlist".
+        { iNext; by iFrame "# ∗". }
+        iDestruct "Hlist" as (L' L1 L2) "(Hpt & >%Hsplit & >%Hsort' & >%Hperm' & Himp)".
+
+        iDestruct (own_valid_2 with "Hown_frac Hown_frag") 
+          as %HsubS%frac_auth_included_total%gset_included.
+
+        assert (key ∉ Skeys') as Hnin'.
+        {
+          intros Hfalse.
+          rewrite -elem_of_elements Hequiv' elem_of_list_In -Hperm in_map_iff in Hfalse.
+          destruct Hfalse as [x [Hkey Hin]].
+          
+          apply (sorted_node_lt_nin L1 L2 pred succ x).
+          { rewrite -Hsplit //. }
+          { rewrite Hkey; lia. }
+          rewrite -Hsplit. apply in_or_app; right. apply in_or_app; by left.
+        }
+
+        assert (key ∉ Skeys) as Hnin.
+        {
           intros Hfalse.
           rewrite -elem_of_elements Hequiv elem_of_list_In in_map_iff in Hfalse.
           destruct Hfalse as [x [Hkey Hin]].
@@ -248,53 +161,29 @@ Module AddSpec (Params: SKIP_LIST_PARAMS).
           rewrite -Hsplit. apply in_or_app; right. apply in_or_app; by left.
         }
 
-        iMod ("Hclose" with "[Hown_auth Hown_frac Hlist]") as "_".
-        { iNext; iExists S, L; by iFrame. }
-        clear Hperm Hsort Hpred_range HsubS S L.
-
-        iModIntro; wp_pures.
-        rewrite (fold_rep_to_node (key, Some l', None, lk)).
-        set (new := (key, Some l', None, lk)).
-        
-        wp_bind (Store _ _).
-        iInv lvlN as (S L) "(>%Hperm & >%Hsort & Hown_auth & Hown_frac & Hlist)" "Hclose".
-        iMod "Hown_auth"; iMod "Hown_frac".
-
-        iAssert ⌜ pred = head ∨ In pred L ⌝%I
-          with "[Hown_auth Hown_pred]" as %Hpred_range.
-        {
-          iDestruct "Hown_pred" as "[Heq|Hown]"; first by iLeft.
-          iDestruct (own_valid_2 with "Hown_auth Hown") 
-            as %[Hvalid%gset_included]%auth_both_valid_discrete.
-          iPureIntro; right. 
-          rewrite -elem_of_list_In Hperm elem_of_elements.
-          set_solver.
-        }
-
-        rewrite (list_equiv_insert head pred new succ L l l' γ'); first last.
-        { done. }
-        { auto. }
-        { rewrite /node_key//=; rewrite /node_key in Hrange'; rewrite /node_key in Hneq; lia. }
-        { rewrite /node_key//=; lia. }
-
         iMod (own_update with "Hown_auth") as "[Hown_auth Hown_auth_frag]".
         { apply auth_update_alloc, (gset_local_update_union _ _ {[ new ]}). }
+        assert (ε ∪ {[ new ]} = {[ new ]}) as -> by set_solver.
+
         iMod (own_update_2 with "Hown_frac Hown_frag") as "[Hown_frac Hown_frac_frag]".
         { apply frac_auth_update, (gset_local_update_union _ _ {[ new ]}). }
 
-        iDestruct ("Hlist" with "[Hpt Hpt' Hlock]") as "Hlist".
-        { iNext; by iFrame "# ∗". }
-        iDestruct "Hlist" as (L') "(Hpt & Hsort & Hperm & Himp)".
-        iMod "Hsort" as %Hsort'; iMod "Hperm" as %Hperm'; iMod "Hpt".
+        rewrite (gset_union_diff key); first last.
+        { done. }
+        { rewrite Zlt_range_spec; lia. }
+        rewrite -gset_disj_union; last set_solver.
+        iDestruct "Hown_toks" as "(Hown_toks & Hown_tok)".
+        
         wp_store.
-
         iDestruct "Hpt" as "(Hpt & Hpt_dup)".
-        iMod ("Hclose" with "[Hpt_dup Himp Hown_auth Hown_frac]") as "_".
+        iPoseProof ("Himp" with "Hpt_dup") as "Hlist".
+        iMod ("Hclose" with "[Hlist Hown_auth Hown_frac Hown_toks]") as "_".
         {
-          iNext. iExists _, L'. 
-          iPoseProof ("Himp" with "Hpt_dup") as "Hlist".
-          iFrame. iPureIntro. split; last done.
-
+          iNext; iExists (S ∪ {[ new ]}), (Skeys' ∪ {[ key ]}), L'.
+          iFrame. iSplit; last first. iSplit; first done.
+          by (iPureIntro; apply key_equiv_insert_nin).
+          
+          iPureIntro.
           apply NoDup_Permutation.
           { 
             apply node_rep_sorted_app in Hsort'; destruct Hsort' as [_ Hsort']. 
@@ -322,12 +211,205 @@ Module AddSpec (Params: SKIP_LIST_PARAMS).
         { iFrame "# ∗"; iExists new; iFrame. }
         iIntros "_". wp_pures. 
         iModIntro. iApply "HΦ".
-        iSplit; last by iRight.
-        iExists (Sfrag ∪ {[new]}).
+        iSplitR "Hown_tok Hown_auth_frag"; last by (iRight; iFrame).
+        iExists (Sfrag ∪ {[ new ]}).
         iFrame "# ∗". iPureIntro.
         apply key_equiv_insert_nin; auto.
+    Qed.
 
-        Unshelve. auto. (* Why ;-; *)
+    Theorem insert_spec (curr down head: node_rep) (key: Z) 
+      (q: frac) (Stop Sbot: gset Z) (top bot: lazy_gname) :
+      INT_MIN < key < INT_MAX →
+      {{{
+        is_lazy_list lvlN head q Stop top (from_sub_list bot)
+        ∗
+        (⌜ curr = head ⌝ ∨ own (s_auth top) (◯ {[ curr ]}))
+        ∗
+        ⌜ node_key curr < key ⌝
+        ∗ 
+        ⌜ node_key down = key ⌝
+        ∗ 
+        own (s_auth bot) (◯ {[ down ]})
+        ∗ 
+        own (s_toks bot) (GSet {[ node_key down ]})
+      }}}
+        insert (rep_to_node curr) #key (rep_to_node down)
+      {{{ v new, RET v;
+        is_lazy_list lvlN head q (Stop ∪ {[ key ]}) top (from_sub_list bot)
+        ∗
+        ⌜ v = SOMEV (rep_to_node new) ⌝ 
+        ∗ 
+        ⌜ node_key new = key ⌝
+        ∗ 
+        own (s_auth top) (◯ {[ new ]})
+        ∗ 
+        own (s_toks top) (GSet {[ node_key new ]})
+      }}}.
+    Proof.
+      iIntros (Hkey_range Φ) "(Hlazy & #Hown_curr & %Hrange & %Hdown & #Hown_down & Hown_tok) HΦ".
+      iDestruct "Hlazy" as (Sfrag) "(%Hequiv & Hown_frag & #Hinv)".
+      wp_lam. wp_let. wp_let.
+
+      wp_apply findLock_spec.
+      { iFrame "#". iPureIntro; lia. }
+      iIntros (pred succ) "(%Hrange' & #Hown_pred & #Hown_succ & Hlock)".
+      iDestruct "Hlock" as (l γ) "(%Hsome & #Hlock & Hpt & Hlocked)".
+
+      wp_pures. wp_lam. wp_pures.
+      rewrite Hsome; wp_match.
+      wp_load. wp_let. 
+      wp_alloc l' as "Hpt'". wp_let.
+      wp_alloc l'' as "Hpt''". wp_let.
+      iDestruct "Hpt'" as "(Hpt' & Hpt'_dup)".
+      
+      wp_apply (newlock_spec (node_inv l') with "[Hpt'_dup]").
+      { iExists succ; iFrame. }
+      iIntros (lk) "#Hlock'". iDestruct "Hlock'" as (γ') "Hlock'".
+
+      wp_bind (InjR _).
+      iInv lvlN as (S Skeys' L) "(>%Hperm & >%Hsort & >%Hequiv' & Hown_auth & Hown_frac & Hown_toks & Hlist)" "Hclose".
+      wp_inj.
+
+      iAssert ⌜ key ≠ node_key succ ⌝%I
+        with "[Hown_auth Hown_succ Hown_tok Hlist]" as %Hneq.
+      {
+        iDestruct "Hown_succ" as "[Hown|%Heq]"; last first.
+        { iPureIntro; rewrite Heq /node_key /=; lia. } 
+
+        iDestruct (own_valid_2 with "Hown_auth Hown") 
+          as %[Hvalid%gset_included]%auth_both_valid_discrete.
+        assert (succ ∈ S) by set_solver.
+
+        rewrite list_equiv_invert_L; last first.
+        { by rewrite -elem_of_list_In Hperm elem_of_elements. }
+        iDestruct "Hlist" as (? ? ? ? ? ) "(_ & _ & _ & _ & _ & HP & _)".
+        iDestruct "HP" as (? ?) "(_ & _ & _ & Hown_tok' & %Hsucc)".
+
+        iDestruct (own_valid_2 with "Hown_tok Hown_tok'") as 
+          %Hdisj%gset_disj_valid_op.
+        iPureIntro; set_solver.
+      }
+
+      iMod ("Hclose" with "[Hlist Hown_auth Hown_frac Hown_toks]") as "_".
+      { iNext; iExists S, Skeys', L; by iFrame "# ∗". }
+      clear Hperm Hsort Hequiv' S Skeys' L.
+
+      iModIntro; wp_pures.
+      set (new := (key, Some l', Some l'', lk)).
+      rewrite (fold_rep_to_node new).
+      
+      wp_bind (Store _ _).
+      iInv lvlN as (S Skeys' L) "(>%Hperm & >%Hsort & >%Hequiv' & >Hown_auth & >Hown_frac & Hown_toks & Hlist)" "Hclose".
+
+      iAssert ⌜ pred = head ∨ In pred L ⌝%I
+        with "[Hown_auth Hown_pred]" as %Hpred_range.
+      {
+        iDestruct "Hown_pred" as "[Heq|Hown]"; first by iLeft.
+        iDestruct (own_valid_2 with "Hown_auth Hown") 
+          as %[Hvalid%gset_included]%auth_both_valid_discrete.
+        iPureIntro; right. 
+        rewrite -elem_of_list_In Hperm elem_of_elements.
+        set_solver.
+      }
+
+      rewrite (list_equiv_insert head pred new succ L l l' γ'); first last.
+      { done. }
+      { auto. }
+      { assert (node_key new = key) as -> by auto; lia. }
+      { rewrite /node_key/=; lia. }
+
+      iDestruct ("Hlist" with "[Hpt Hpt' Hpt'' Hlock Hown_tok]") as "Hlist".
+      { 
+        iNext; iFrame "# ∗". 
+        iSplit; first done. iSplit; first done.
+        iExists l'', down. by iFrame "# ∗".
+      }
+      iDestruct "Hlist" as (L' L1 L2) "(Hpt & >%Hsplit & >%Hsort' & >%Hperm' & Himp)".
+
+      iDestruct (own_valid_2 with "Hown_frac Hown_frag") 
+        as %HsubS%frac_auth_included_total%gset_included.
+      
+      assert (key ∉ Skeys') as Hnin'.
+      {
+        intros Hfalse.
+        rewrite -elem_of_elements Hequiv' elem_of_list_In -Hperm in_map_iff in Hfalse.
+        destruct Hfalse as [x [Hkey Hin]].
+        
+        apply (sorted_node_lt_nin L1 L2 pred succ x).
+        { rewrite -Hsplit //. }
+        { rewrite Hkey; lia. }
+        rewrite -Hsplit. apply in_or_app; right. apply in_or_app; by left.
+      }
+
+      assert (key ∉ Stop) as Hnin.
+      {
+        intros Hfalse.
+        rewrite -elem_of_elements Hequiv elem_of_list_In in_map_iff in Hfalse.
+        destruct Hfalse as [x [Hkey Hin]].
+        rewrite -elem_of_list_In elem_of_elements in Hin.
+        assert (x ∈ S) as HinS by set_solver; clear Hin.
+        rewrite -elem_of_elements -Hperm elem_of_list_In in HinS.
+        
+        apply (sorted_node_lt_nin L1 L2 pred succ x).
+        { rewrite -Hsplit //. }
+        { rewrite Hkey; lia. }
+        rewrite -Hsplit. apply in_or_app; right. apply in_or_app; by left.
+      }
+
+      iMod (own_update with "Hown_auth") as "[Hown_auth Hown_auth_frag]".
+      { apply auth_update_alloc, (gset_local_update_union _ _ {[ new ]}). }
+      assert (ε ∪ {[ new ]} = {[ new ]}) as -> by set_solver.
+
+      iMod (own_update_2 with "Hown_frac Hown_frag") as "[Hown_frac Hown_frac_frag]".
+      { apply frac_auth_update, (gset_local_update_union _ _ {[ new ]}). }
+
+      rewrite (gset_union_diff key); first last.
+      { done. }
+      { rewrite Zlt_range_spec; lia. }
+      rewrite -gset_disj_union; last set_solver.
+      iDestruct "Hown_toks" as "(Hown_toks & Hown_tok)".
+
+      wp_store.
+      iDestruct "Hpt" as "(Hpt & Hpt_dup)".
+      iMod ("Hclose" with "[Hpt_dup Himp Hown_auth Hown_frac Hown_toks]") as "_".
+      {
+        iNext; iExists (S ∪ {[ new ]}), (Skeys' ∪ {[ key ]}), L'. 
+        iPoseProof ("Himp" with "Hpt_dup") as "Hlist".
+        iFrame. iSplit; last first. iSplit; first done.
+        by (iPureIntro; apply key_equiv_insert_nin).
+        
+        iPureIntro.
+        apply NoDup_Permutation.
+        { 
+          apply node_rep_sorted_app in Hsort'; destruct Hsort' as [_ Hsort']. 
+          apply node_rep_sorted_app in Hsort'; destruct Hsort' as [Hsort' _].
+          by apply sorted_node_lt_no_dup.
+        } 
+        { apply NoDup_elements. }
+
+        simpl in Hperm'; apply Permutation_cons_inv in Hperm'.
+        intros x; split.
+        - rewrite elem_of_elements Hperm' elem_of_list_In.
+          intros Hin. destruct Hin as [Heq|Hin].
+          * set_solver.
+          * apply elem_of_union_l. 
+            by rewrite -elem_of_elements -Hperm elem_of_list_In.
+        - rewrite elem_of_elements Hperm'. 
+          intros Hin. apply elem_of_union in Hin as [Hin|Heq].
+          * rewrite elem_of_list_In. right.
+            by rewrite -elem_of_list_In Hperm elem_of_elements.
+          * set_solver.
+      }
+
+      iModIntro. wp_pures. wp_lam. wp_pures.
+      wp_apply (release_spec with "[Hlock Hpt Hlocked]"); first done.
+      { iFrame "# ∗"; iExists new; iFrame. }
+      iIntros "_". wp_pures. 
+      iModIntro. iApply "HΦ".
+      iSplitR "Hown_tok Hown_auth_frag"; last by iFrame.
+      iExists (Sfrag ∪ {[ new ]}).
+      iFrame "# ∗". iPureIntro.
+      apply key_equiv_insert_nin; auto.
     Qed.
 
   End Proofs.
